intermediate/Veritas.Intermediate.VerifySKC.fst
@@ -1,17 +1,26 @@
-module Veritas.Intermediate.Verifier
-open Veritas.Intermediate.Common
+module Veritas.Intermediate.VerifySKC
+open Veritas.Intermediate.Logs
 open Veritas.Intermediate.Store
 
-module R = Veritas.Record
-module K = Veritas.Key
+module BT = Veritas.BinTree
+module FE = FStar.FunctionalExtensionality
 module H = Veritas.Hash
+module K = Veritas.Key
 module MH = Veritas.MultiSetHash
 module MHD = Veritas.MultiSetHashDomain
-module BT = Veritas.BinTree
-module V = Veritas.Verifier
+module R = Veritas.Record
 module SA = Veritas.SeqAux
+module V = Veritas.Verifier
+module VT = Veritas.Verifier.Thread
 
-(* id     : thread id
+let data_key = K.data_key
+let merkle_key = K.merkle_key
+let data_value = R.data_value 
+let thread_id = V.thread_id
+let timestamp = MHD.timestamp
+
+(* Thread-local state
+   id     : thread id
    st     : thread local store
    clock  : current timestamp
    hadd   : add set hash
@@ -61,37 +70,40 @@ let update_thread_hevict (vs:vtls {Valid? vs}) (hevict:MH.ms_hash_value): vtls =
   match vs with
   | Valid id st clock hadd _ -> Valid id st clock hadd hevict
 
-let vget (s:slot_id) (v:data_value) (vs: vtls {Valid? vs}): vtls =
+let vget (s:slot_id) (k:data_key) (v:data_value) (vs: vtls {Valid? vs}) : vtls =
   let st = thread_store vs in
   (* check store contains slot s *)
   if not (contains_record st s) then Failed
-  (* check stored value is v *)
-  else let v' = get_value_at st s in
-       if not (R.DVal? v') then Failed
+  (* check stored key and value *)
+  else let k' = get_key_at st s in
+       let v' = get_value_at st s in
+       if k' <> k then Failed
+       else if not (R.DVal? v') then Failed
        else if R.to_data_value v' <> v then Failed
        else vs
 
-let vput (s:slot_id) (v:data_value) (vs: vtls {Valid? vs}): vtls =
+let vput (s:slot_id) (k:data_key) (v:data_value) (vs: vtls {Valid? vs}) : vtls =
   let st = thread_store vs in
   (* check store contains slot s *)
   if not (contains_record st s) then Failed
-  (* check stored key is a data key *)
-  else if not (K.is_data_key (get_key_at st s)) then Failed
+  (* check stored key is k *)
+  else if get_key_at st s <> k then Failed
   else update_thread_store vs (update_record_value st s (R.DVal v))
 
-let vaddm (s:slot_id) (r:record) (s':slot_id) (vs: vtls {Valid? vs}): vtls =
+let vaddm (s:slot_id) (r:R.record) (s':slot_id) (k0':merkle_key) (vs: vtls {Valid? vs}): vtls =
   let st = thread_store vs in
   if not (s < Seq.length st.data) then Failed
   (* check store contains slot s' *)
   else if not (contains_record st s') then Failed
   else
-    let k = Record?.k r in
-    let v = Record?.v r in
+    let (k,v) = r in
     let k' = get_key_at st s' in
     let v' = get_value_at st s' in
     let a' = get_add_method_at st s' in 
+    (* check key is consistent with argument *)
+    if k' <> k0' then Failed
     (* check k is a proper desc of k' *)
-    if not (BT.is_proper_desc k k') then Failed
+    else if not (BT.is_proper_desc k k') then Failed
     (* check store does not contain slot s *)
     else if contains_record st s then Failed
     (* check type of v is consistent with k *)
@@ -139,7 +151,7 @@ let is_instore_madd (st: vstore) (k: key): bool =
   contains_key st k && 
   add_method_of st k = V.MAdd
 
-let has_instore_merkle_desc (st: vstore) (k:key{contains_key st k}): bool = 
+let has_instore_merkle_desc (st:vstore) (k:key{contains_key st k}): bool = 
   if K.is_data_key k then false
   else 
     let v = R.to_merkle_value (value_of st k) in
@@ -148,7 +160,7 @@ let has_instore_merkle_desc (st: vstore) (k:key{contains_key st k}): bool =
     R.Desc? ld && is_instore_madd st (R.Desc?.k ld) || 
     R.Desc? rd && is_instore_madd st (R.Desc?.k rd)
 
-let vevictm (s s':slot_id) (vs: vtls {Valid? vs}): vtls = 
+let vevictm (s:slot_id) (k0:key) (s':slot_id) (k0':merkle_key) (vs: vtls {Valid? vs}): vtls = 
   let st = thread_store vs in
   (* check store contains s and s' *)
   if not (contains_record st s && contains_record st s') then Failed
@@ -159,8 +171,11 @@ let vevictm (s s':slot_id) (vs: vtls {Valid? vs}): vtls =
     let k' = get_key_at st s' in
     let v' = get_value_at st s' in
     let a' = get_add_method_at st s' in
+    (* check keys are consistent with arguments *)
+    if k <> k0 then Failed
+    else if k' <> k0' then Failed
     (* check k is a proper descendent of k' *)
-    if not (BT.is_proper_desc k k') then Failed
+    else if not (BT.is_proper_desc k k') then Failed
     (* check k does not have a child in the store *)
     else if (
               lemma_contains_key st s k; 
@@ -179,14 +194,13 @@ let vevictm (s s':slot_id) (vs: vtls {Valid? vs}): vtls =
                           let st_upd = evict_record (update_record_value st s' (R.MVal v'_upd)) s in
                          update_thread_store vs st_upd
 
-let vaddb (s:slot_id) (r:record) (t:timestamp) (j:thread_id) (vs:vtls {Valid? vs}): vtls = 
+let vaddb (s:slot_id) (r:R.record) (t:timestamp) (j:thread_id) (vs:vtls {Valid? vs}): vtls = 
   let st = thread_store vs in 
   if not (s < Seq.length st.data) then Failed
   (* epoch of timestamp of last evict *)
   else 
     let e = MHD.MkTimestamp?.e t in
-    let k = Record?.k r in
-    let v = Record?.v r in
+    let (k,v) = r in
     (* check value type consistent with key k *)
     if not (R.is_value_of k v) then Failed
     (* check store contains slot s *)
@@ -207,7 +221,7 @@ let vaddb (s:slot_id) (r:record) (t:timestamp) (j:thread_id) (vs:vtls {Valid? vs
       let st_upd2 = add_record st_upd s k v V.BAdd in
       update_thread_store vs_upd2 st_upd2
 
-let vevictb (s:slot_id) (t:timestamp) (vs:vtls {Valid? vs}): vtls = 
+let vevictb (s:slot_id) (k0:key) (t:timestamp) (vs:vtls {Valid? vs}): vtls = 
   let clock = thread_clock vs in
   let e = MHD.MkTimestamp?.e t in
   let st = thread_store vs in
@@ -216,8 +230,10 @@ let vevictb (s:slot_id) (t:timestamp) (vs:vtls {Valid? vs}): vtls =
   else
     let k = get_key_at st s in
     let v = get_value_at st s in
+    (* check key is consistent with argument *)
+    if k <> k0 then Failed
     (* check key at s is not root *)
-    if k = BT.Root then Failed
+    else if k = BT.Root then Failed
     (* check time of evict < current time *)
     else if not (MHD.ts_lt clock t) then Failed
     (* check s was added through blum *)  
@@ -238,7 +254,7 @@ let vevictb (s:slot_id) (t:timestamp) (vs:vtls {Valid? vs}): vtls =
       let st_upd = evict_record st s in
       update_thread_store vs_upd2 st_upd
 
-let vevictbm (s s':slot_id) (t:timestamp) (vs:vtls {Valid? vs}): vtls = 
+let vevictbm (s:slot_id) (k0:key) (s':slot_id) (k0':merkle_key) (t:timestamp) (vs:vtls {Valid? vs}): vtls = 
   let st = thread_store vs in
   (* check store contains s and s' *)
   if not (contains_record st s && contains_record st s') then Failed
@@ -246,8 +262,11 @@ let vevictbm (s s':slot_id) (t:timestamp) (vs:vtls {Valid? vs}): vtls =
     let k = get_key_at st s in
     let k' = get_key_at st s' in
     let v' = get_value_at st s' in
+    (* check keys are consistent with arguments *)
+    if k <> k0 then Failed
+    else if k' <> k0' then Failed
     (* check k is a proper desc of k' *)
-    if not (BT.is_proper_desc k k') then Failed
+    else if not (BT.is_proper_desc k k') then Failed
     (* check s was added through merkle *)
     else if get_add_method_at st s <> V.MAdd then Failed  
     (* check k has no children in the store *)
@@ -265,28 +284,26 @@ let vevictbm (s s':slot_id) (t:timestamp) (vs:vtls {Valid? vs}): vtls =
                           else
                             let v'_upd = V.update_merkle_value v' d k h2 true in
                             let st_upd = update_record_value st s' (R.MVal v'_upd) in
-                            vevictb s t (update_thread_store vs st_upd)
+                            vevictb s k0 t (update_thread_store vs st_upd)
 
 (* thread-level verification step
    (following the defn in Veritas.Verifier) *)
 let t_verify_step (vs:vtls)
-                  (e:vlog_entry): vtls =                           
+                  (e:logSK_entry): vtls =                           
   match vs with
   | Failed -> Failed (* could check the is_map flag here *)
   | _ ->
     match e with
-    | Get s v -> vget s v vs
-    | Put s v -> vput s v vs
-    | AddM s r s'  -> vaddm s r s' vs
-    | EvictM s s' -> vevictm s s' vs
-    | AddB s r t j -> vaddb s r t j vs
-    | EvictB s t -> vevictb s t vs
-    | EvictBM s s' t -> vevictbm s s' t vs
-
-let vlog = Seq.seq vlog_entry
+    | Get_SK s k v -> vget s k v vs
+    | Put_SK s k v -> vput s k v vs
+    | AddM_SK s r s' k'  -> vaddm s r s' k' vs
+    | EvictM_SK s k s' k' -> vevictm s k s' k' vs
+    | AddB_SK s r t j -> vaddb s r t j vs
+    | EvictB_SK s k t -> vevictb s k t vs
+    | EvictBM_SK s k s' k' t -> vevictbm s k s' k' t vs
 
 (* verify a log from a specified initial state *)
-let rec t_verify_aux (vs:vtls) (l:vlog): Tot vtls
+let rec t_verify_aux (vs:vtls) (l:logSK): Tot vtls
   (decreases (Seq.length l)) =
   let n = Seq.length l in
   if n = 0 then vs
@@ -296,7 +313,7 @@ let rec t_verify_aux (vs:vtls) (l:vlog): Tot vtls
     let e' = Seq.index l (n - 1) in
     t_verify_step vs' e'
 
-// TODO: what should the initial size be? a parameter? some contant?
+// TODO: what should the initial size be?
 let empty_store:vstore = { data=Seq.create 10 None; is_map=true }
 
 (* initialize verifier state *)
@@ -304,19 +321,173 @@ let init_thread_state (id:thread_id): vtls =
   let vs = Valid id empty_store (MHD.MkTimestamp 0 0) MHD.empty_hash_value MHD.empty_hash_value in  
   if id = 0 then
     let st0 = thread_store vs in
-    // TODO: where should we stick the root?
     let st0_upd = add_record st0 0 BT.Root (R.init_value BT.Root) V.MAdd in
     update_thread_store vs st0_upd    
   else vs
 
-let t_verify (id:thread_id) (l:vlog): vtls = 
+let t_verify (id:thread_id) (l:logSK): vtls = 
   t_verify_aux (init_thread_state id) l 
 
-let verify (id:thread_id) (l:vlog): vtls =
+let verify (id:thread_id) (l:logSK): vtls =
   let vs = t_verify id l in
   if Valid? vs
   then if thread_store_is_map vs then vs else Failed
   else Failed
 
-let verifiable (id:thread_id) (l: vlog): bool =
+let verifiable (id:thread_id) (l: logSK): bool =
   Valid? (verify id l)
+
+(** Proofs **)
+
+module Spec = Veritas.Verifier
+
+(* Relation between stores *)
+let store_rel (st:vstore) (st':Spec.vstore) : Type = 
+  st.is_map /\ FE.feq st' (as_map st)
+
+(* Relation between thread-local states *)
+let vtls_rel (vs:vtls) (vs':Spec.vtls) : Type =
+  match vs, vs' with
+  // either both runs failed
+  | Failed, Spec.Failed -> True
+  // or both are valid and the stores are related
+  | Valid id st clk ha he, Spec.Valid id' st' clk' _ ha' he' ->
+       store_rel st st' /\ 
+       // other fields related by equality  
+       id = id' /\ clk = clk' /\ ha = ha' /\ he = he'   
+  // or the spec run failed, but the store of vs is not a map
+  | Valid _ st _ _ _, _ -> not st.is_map
+  | _, _ -> False
+
+(* Relation between a slot and key *)
+let is_key_of (vs: vtls {Valid? vs}) (s:slot_id) (k:key) =
+  let st = thread_store vs in slot_key_equiv st s k
+
+let lemma_contains_record_store_contains 
+      (st:vstore) 
+      (s:slot_id) 
+      (st':Spec.vstore{store_rel st st'}) 
+      (k:key{slot_key_equiv st s k})
+  : Lemma (contains_record st s = Spec.store_contains st' k)
+  = admit()
+
+let lemma_get_value_at_stored_value
+      (st:vstore) 
+      (s:slot_id) 
+      (st':Spec.vstore{store_rel st st'}) 
+      (k:data_key{slot_key_equiv st s k /\ Spec.store_contains st' k})
+  : Lemma (get_value_at st s = Spec.stored_value st' k)
+  = admit()
+
+let lemma_update_record_value_update_store
+      (st:vstore) 
+      (s:slot_id) 
+      (st':Spec.vstore{store_rel st st'}) 
+      (k:data_key{slot_key_equiv st s k /\ Spec.store_contains st' k})
+      (v:data_value)
+  : Lemma (store_rel (update_record_value st s (R.DVal v)) (Spec.update_store st' k (R.DVal v)))
+  = admit()
+
+let lemma_vget_simulates_spec 
+      (vs:vtls{Valid? vs})
+      (vs':Spec.vtls{Spec.Valid? vs'})
+      (s:slot_id)
+      (k:data_key)
+      (v:data_value)
+  : Lemma (requires (vtls_rel vs vs' /\ is_key_of vs s k))
+          (ensures (vtls_rel (vget s k v vs) (Spec.vget k v vs')))
+  = let st = thread_store vs in
+    let st' = Spec.thread_store vs' in
+    lemma_contains_record_store_contains st s st' k;
+    lemma_get_value_at_stored_value st s st' k
+
+let lemma_vput_simulates_spec 
+      (vs:vtls{Valid? vs}) 
+      (vs':Spec.vtls{Spec.Valid? vs'}) 
+      (s:slot_id) 
+      (k:data_key) 
+      (v:data_value) 
+  : Lemma (requires (vtls_rel vs vs' /\ is_key_of vs s k))
+          (ensures (vtls_rel (vput s k v vs) (Spec.vput k v vs'))) 
+  = let st = thread_store vs in
+    let st' = Spec.thread_store vs' in
+    lemma_contains_record_store_contains st s st' k;
+    lemma_update_record_value_update_store st s st' k v
+
+let lemma_vaddm_simulates_spec 
+      (vs:vtls{Valid? vs}) 
+      (vs':Spec.vtls{Spec.Valid? vs'}) 
+      (s s':slot_id)
+      (r:R.record)
+      (k':merkle_key)  
+  : Lemma (requires (vtls_rel vs vs'))
+          (ensures (vtls_rel (vaddm s r s' k' vs) (Spec.vaddm r k' vs'))) 
+  = admit()
+
+let lemma_vevictm_simulates_spec 
+      (vs:vtls{Valid? vs}) 
+      (vs':Spec.vtls{Spec.Valid? vs'}) 
+      (s s':slot_id)
+      (k:key)
+      (k':merkle_key)  
+  : Lemma (requires (vtls_rel vs vs'))
+          (ensures (vtls_rel (vevictm s k s' k' vs) (Spec.vevictm k k' vs'))) 
+  = admit()
+
+let lemma_vaddb_simulates_spec 
+      (vs:vtls{Valid? vs}) 
+      (vs':Spec.vtls{Spec.Valid? vs'}) 
+      (s:slot_id)
+      (r:R.record)
+      (t:timestamp)
+      (j:thread_id)
+  : Lemma (requires (vtls_rel vs vs'))
+          (ensures (vtls_rel (vaddb s r t j vs) (Spec.vaddb r t j vs'))) 
+  = admit()
+
+let lemma_vevictb_simulates_spec 
+      (vs:vtls{Valid? vs}) 
+      (vs':Spec.vtls{Spec.Valid? vs'}) 
+      (s:slot_id)
+      (k:key)
+      (t:timestamp)
+  : Lemma (requires (vtls_rel vs vs'))
+          (ensures (vtls_rel (vevictb s k t vs) (Spec.vevictb k t vs'))) 
+  = admit()
+
+let lemma_vevictbm_simulates_spec 
+      (vs:vtls{Valid? vs}) 
+      (vs':Spec.vtls{Spec.Valid? vs'}) 
+      (s s':slot_id)
+      (k:key)
+      (k':merkle_key)
+      (t:timestamp)
+  : Lemma (requires (vtls_rel vs vs'))
+          (ensures (vtls_rel (vevictbm s k s' k' t vs) (Spec.vevictbm k k' t vs'))) 
+  = admit()
+
+(* Relation between logs *)
+let log_rel  (l:logSK) (l':logK) : Type 
+  = skc l /\ drop_slots l = l'
+
+(* given a log with only slots, add consistent keys *)
+
+(* given a log with keys and slots, check that the key accesses are consistent with evicts and adds *)
+
+let lemma_t_verify_simulates_spec (id:thread_id) (l:logSK) (l':logK)
+  : Lemma (requires (log_rel l l'))
+          (ensures (vtls_rel (t_verify id l) (Spec.t_verify id l')))
+  = admit()
+
+(* For any log, the intermediate implementation will verify 
+   iff the the spec implementation does. *)
+
+let lemma_verifiable_simulates_spec (id:thread_id) (l:logSK) (l':logK)
+  : Lemma (requires (log_rel l l'))
+          (ensures (let tl : VT.thread_id_vlog = (id,l') in
+                    verifiable id l = VT.verifiable tl))
+  = lemma_t_verify_simulates_spec id l l';
+    let vs = t_verify id l in
+    if Valid? vs
+    then if not (thread_store_is_map vs) 
+    then admit()
