intermediate/Veritas.Intermediate.Logs.fst
@@ -1,0 +1,68 @@
+module Veritas.Intermediate.Logs
+
+module K = Veritas.Key
+module MHD = Veritas.MultiSetHashDomain
+module R = Veritas.Record
+module SA = Veritas.SeqAux
+module V = Veritas.Verifier
+
+let slot_id = Veritas.Intermediate.Store.slot_id
+let key = K.key
+let data_key = K.data_key
+let merkle_key = K.merkle_key
+let value = R.value
+let data_value = R.data_value
+let record = R.record
+let timestamp = MHD.timestamp
+let thread_id = V.thread_id
+
+(* Definitions of different styles of verifier logs.
+   - logK : contains only key references (defined in Veritas.Verifier)
+   - logSK: contains both slot and key references
+   - logS: contains only slot references *)
+
+let logK_entry = V.vlog_entry
+let logK = V.vlog
+
+noeq
+type logSK_entry =
+  | Get_SK: s:slot_id -> k:data_key -> v:data_value -> logSK_entry
+  | Put_SK: s:slot_id -> k:data_key -> v:data_value -> logSK_entry
+  | AddM_SK: s:slot_id -> r:record -> s':slot_id -> k':merkle_key -> logSK_entry
+  | EvictM_SK: s:slot_id -> k:key -> s':slot_id -> k':merkle_key -> logSK_entry
+  | AddB_SK: s:slot_id -> r:record -> t:timestamp -> j:thread_id -> logSK_entry
+  | EvictB_SK: s:slot_id -> k:key -> t:timestamp -> logSK_entry
+  | EvictBM_SK: s:slot_id -> k:key -> s':slot_id -> k':merkle_key -> t:timestamp -> logSK_entry
+             
+let logSK = Seq.seq logSK_entry
+
+noeq
+type logS_entry =
+  | Get_S: s:slot_id -> v:data_value -> logS_entry
+  | Put_S: s:slot_id -> v:data_value -> logS_entry
+  | AddM_S: s:slot_id -> r:record -> s':slot_id -> logS_entry
+  | EvictM_S: s:slot_id -> s':slot_id -> logS_entry
+  | AddB_S: s:slot_id -> r:record -> t:timestamp -> j:thread_id -> logS_entry
+  | EvictB_S: s:slot_id -> t:timestamp -> logS_entry
+  | EvictBM_S: s:slot_id -> s':slot_id -> t:timestamp -> logS_entry
+
+let logS = Seq.seq logS_entry
+
+let drop_slots_aux (e:logSK_entry) :logK_entry =
+  match e with
+  | Get_SK _ k v -> V.Get k v
+  | Put_SK _ k v -> V.Put k v
+  | AddM_SK _ r _ k' -> V.AddM r k'
+  | EvictM_SK _ k _ k' -> V.EvictM k k'
+  | AddB_SK _ r t j -> V.AddB r t j
+  | EvictB_SK _ k t -> V.EvictB k t
+  | EvictBM_SK _ k _ k' t -> V.EvictBM k k' t
+  
+let drop_slots (l:logSK) : logK 
+  = SA.map drop_slots_aux l
+
+// likely similar to EAC: check that for every "OP s k ...", k is the last key added at slot s, and has not been evicted 
+let skc (l:logSK) : Type = admit()
+
+// add keys in a way that satisfies skc
+let add_consistent_keys (l:logS) : logSK = admit()
